isomorphism_refl and symm. need bijective μ for trans

src/Rdf.v
@@ -19,78 +19,113 @@ Section rdf.
                        }.
 
   Definition eqb_rdf (g1 g2 : rdf_graph) : bool :=
-    eqseq (graph g1) (graph g2).
+    (graph g1) == (graph g2).
+
+  Lemma eqb_rdf_refl (g : rdf_graph) : eqb_rdf g g.
+  Proof. by rewrite /eqb_rdf. Qed.
+
+  Lemma eqb_rdf_symm (g1 g2 : rdf_graph) : eqb_rdf g1 g2 = eqb_rdf g2 g1.
+  Proof. by rewrite /eqb_rdf. Qed.
 
   Lemma eq_ir : forall (g1 g2: seq triple)
                   (geq : g1 = g2)
                   (p : triple -> bool)
                   (fallt : all p g1),
-                  all p g2.
+      all p g2.
   Proof. move=> g1 g2 eqg p fallt. by [rewrite -eqg].
   Qed.
 
-
   Lemma graph_inj : forall (g1 g2: rdf_graph),
-      graph g1 == graph g2 ->
+      eqb_rdf g1 g2 ->
       g1 = g2.
-  Proof. move=> [g1 sib1 pi1 oibl1] [g2 sib2 pi2 oibl2] /= /eqP geq.
-         have: sib2 = (eq_ir geq sib1). apply eq_irrelevance.
-         have: pi2 = (eq_ir geq pi1). apply eq_irrelevance.
-         have: oibl2 = (eq_ir geq oibl1). apply eq_irrelevance. move => eqoibl eqpi eqsib.
-         rewrite eqsib eqpi eqoibl. erewrite <-geq. f_equal; apply eq_irrelevance.
-         Qed.
+  Proof.
+    move=> [g1 sib1 pi1 oibl1] [g2 sib2 pi2 oibl2] /= /eqP /= geq.
+    have eqsib: sib2 = (eq_ir geq sib1);
+      have eqpi : pi2 = (eq_ir geq pi1);
+      have eqoibl: oibl2 = (eq_ir geq oibl1); try apply eq_irrelevance.
+    rewrite eqsib eqpi eqoibl. erewrite <-geq. f_equal; apply eq_irrelevance. 
+  Qed.
   
   Definition rdf_eqP : Equality.axiom eqb_rdf.
   Proof. rewrite /Equality.axiom => x y.
-    apply: (iffP idP) => //= [| ->]; case: x y=> [g1 sib1 pi1 oibl1] [g2 sib2 pi2 oibl2]. move=> /eqP //= geq.
-    apply: graph_inj => //=. by rewrite geq eq_refl.
-    rewrite /eqb_rdf //=. elim g2 => [//|h t IHt]=> //=. rewrite eq_refl //=.
+         apply: (iffP idP) => //= [| ->]; case: x y=> [g1 sib1 pi1 oibl1] [g2 sib2 pi2 oibl2]. apply graph_inj. apply eqb_rdf_refl. 
   Qed.
 
-  Definition relabelingG (g : seq triple) (μ : B -> B) : seq triple :=
-    map (fun t => relabeling t μ) g.
+  Definition relabelingG (μ : B -> B) (g : seq triple) : seq triple :=
+    map (relabeling μ) g.
+
+  Lemma relabelingG_id (g : seq triple) : relabelingG id g = g.
+  Proof. rewrite /relabelingG. apply /eqP. elim g => [//|h t /eqP iht] /=. rewrite relabeling_id. by rewrite iht. Qed.
+  
+  (* map_comp: *)
+  (*   forall [T1 T2 T3 : Type] (f1 : T2 -> T3) (f2 : T1 -> T2) (s : seq T1), *)
+  (*   [seq (f1 \o f2) i | i <- s] = [seq f1 i | i <- [seq f2 i | i <- s]] *)
+
+  Lemma relabelingG_comp (g : seq triple) (μ12 μ23 : B -> B) :
+    relabelingG (μ23 \o μ12) g = (relabelingG μ23 \o (relabelingG μ12)) g.
+  Proof. rewrite /relabelingG /=. elim g => [//|h t iht] /=. rewrite relabeling_comp /=. f_equal; apply iht.
+  Qed.
 
   Lemma relabelingG_preserves_subject_in_IB (g : seq triple) (μ : B -> B) :
     all (fun t => is_in_ib (subject t)) g ->
-    all (fun t => is_in_ib (subject t)) (relabelingG g μ).
+    all (fun t => is_in_ib (subject t)) (relabelingG μ g).
   Proof. move=> /allP sin. apply /allP => [[s p o /= sint pint oint]] => tg. apply sint. 
   Qed.
 
   Lemma relabelingG_preserves_predicate_in_I (g : seq triple) (μ : B -> B) :
     all (fun t => is_in_i (predicate t)) g ->
-    all (fun t => is_in_i (predicate t)) (relabelingG g μ).
+    all (fun t => is_in_i (predicate t)) (relabelingG μ g).
   Proof. move=> /allP pin. apply /allP => [[s p o /= sint pint oint]] => tg . apply pint.
   Qed.
 
   Lemma relabelingG_preserves_object_in_IBL (g : seq triple) (μ : B -> B) :
     all (fun t => is_in_ibl (object t)) g ->
-    all (fun t => is_in_ibl (object t)) (relabelingG g μ).
+    all (fun t => is_in_ibl (object t)) (relabelingG μ g).
   Proof. move=> /allP oin. apply /allP => [[s p o /= sibt pibt oint]] => tg . apply oint.
   Qed.
 
-  Lemma relabel_ (g : seq triple) (μ : B -> B) : (all (fun t => is_in_ib (subject (relabeling t μ))) g) -> all (fun t => is_in_ib (subject t)) (relabelingG g μ).
-  Proof.
-    move=> /all_sigP H. apply /allP => [[s p o sin pin oin]] /= => _. apply sin.
-    Qed.
-
-  Definition relabeling (g : rdf_graph) (μ : B -> B) : rdf_graph :=
+  Definition relabeling (μ : B -> B) (g : rdf_graph): rdf_graph :=
     let (g',siib,pii,oiibl) := g in
     {|
-      graph := relabelingG g' μ;
+      graph := relabelingG μ g';
       subject_in_IB :=  relabelingG_preserves_subject_in_IB μ siib;
       predicate_in_I := relabelingG_preserves_predicate_in_I μ pii;
       object_in_IBL := relabelingG_preserves_object_in_IBL μ oiibl
     |}.
 
-  Definition is_iso (g1 g2 : rdf_graph) (μ : B -> B) : bool :=
-    eqb_rdf g1 (relabeling g2 μ) && eqb_rdf (relabeling g1 μ) g2.
+  Lemma relabeling_id (g : rdf_graph) : relabeling id g = g.
+  Proof. apply graph_inj. case g=> g' sin pin oin. rewrite /relabeling /= /eqP /eqb_rdf /=. by rewrite /eqP relabelingG_id.
+  Qed.
 
-  Definition iso (g1 g2 : rdf_graph):= exists (μ : B -> B), is_iso g1 g2 μ.
+  Lemma relabeling_comp (g : rdf_graph) (μ12 μ23: B -> B) :
+    (relabeling μ23 \o (relabeling μ12)) g = relabeling (μ23 \o μ12) g.
+  Proof. apply graph_inj. rewrite /eqb_rdf. apply /eqP.
+         case g=> g' sin pin oin /=. by rewrite relabelingG_comp.
+  Qed.
 
-  (* Lemma iso_refl : forall (g : rdf_graph), iso g g. *)
-  (* Proof. rewrite /iso /is_iso /relabeling //=. exists id. *)
+  Definition is_iso (g1 g2 : rdf_graph) (μ : B -> B) :=
+    eqb_rdf g1 (relabeling μ g2) && eqb_rdf (relabeling μ g1) g2.
 
+  Definition iso (g1 g2 : rdf_graph):= exists (μ : B -> B),
+      (* (bijective μ) -> *)
+      is_iso g1 g2 μ.
 
+  Lemma iso_refl (g : rdf_graph) : iso g g.
+  Proof. rewrite /iso /is_iso. exists id. by rewrite relabeling_id eqb_rdf_refl.
+  Qed.
+
+  Lemma iso_symm (g1 g2 : rdf_graph) : iso g1 g2 <-> iso g2 g1.
+  Proof. rewrite /iso /is_iso. split=> [[μ] /andP [liso riso]|[μ] /andP [liso riso]];
+                                      exists μ; apply /andP; split; rewrite eqb_rdf_symm; try apply riso; apply liso. Qed.
+
+  Lemma iso_trans (g1 g2 g3: rdf_graph) : iso g1 g2 -> iso g2 g3 -> iso g1 g3.
+  Proof. rewrite /iso /is_iso => [[μ12] /andP [/eqP  eqb12 /eqP eqb21]] [μ23] /andP [/eqP eqb23 /eqP eqb32].
+         exists (μ23 \o μ12). apply /andP. split.
+         apply /eqP. rewrite -relabeling_comp /=.
+         rewrite eqb12. have g2rel: g2 = (relabeling μ23 g3). apply graph_inj. apply /eqP. apply eqb23.
+         rewrite g2rel.
+         (* need bijective μ!!!*)
+  Abort.
 
 End rdf.
 
